okasaki/QueueSig.ml
@@ -1,6 +1,18 @@
 module type Queue =
 sig
-   type 'a queue
+   type 'a queue 
+
+   val empty : 'a queue
+   val is_empty : 'a queue -> bool
+   
+   val snoc : 'a queue -> 'a -> 'a queue
+   val head : 'a queue -> 'a 
+   val tail : 'a queue -> 'a queue
+end
+
+module type QueueBis =
+sig
+   type 'a queue = 'a list
 
    val empty : 'a queue
    val is_empty : 'a queue -> bool
