okasaki/CatenableListImpl_proof.v
@@ -3,58 +3,79 @@ Require Import FuncTactics LibCore.
 Require Import QueueSig_ml QueueSig_proof.
 Require Import CatenableListImpl_ml.
 Require Import CatenableListSig_ml CatenableListSig_proof.
-Require Import BankersQueue_ml.
-Declare Module BankersQueueSpec : QueueSigSpec with Module Q := MLBankersQueue.
-Import BankersQueueSpec.
 
-Module CatenableListImplSpec (* (Q:MLQueue) (QS:QueueSigSpec with Module Q:=Q)*)
-  <: CatenableListSigSpec.
+
+(* todo: move *)
+Lemma Forall2_unique : forall A1 A2 (P:A1->A2->Prop) l L1 L2,
+  (forall x X Y, P x X -> P x Y -> X = Y) -> 
+  Forall2 P l L1 -> Forall2 P l L2 -> L1 = L2.
+Proof.
+  induction l; introv H H1 H2; inverts H1; inverts H2; prove_rep.
+Qed.
+
+Hint Resolve Forall2_unique : rep.
+
+(*todo:move
+Definition rep_from_eq : forall A, Rep A A.
+Proof. intros. apply (Build_Rep eq). congruence. Defined.
+*)
+
+Module CatenableListImplSpec (Q:MLQueueBis) (QS:QueueBisSigSpec with Module Q:=Q) <: CatenableListSigSpec.
 
 (** instantiations *)
 
-Module Import C <: MLCatenableList := MLCatenableListImpl.
-Import MLCatenableListImpl.
+Import Q.
+Module Import C <: MLCatenableList := MLCatenableListImpl Q.
 
 (** invariant *)
 
-Inductive inv : forall `{Rep a A}, cat a -> list A -> Prop :=
-  | inv_empty : forall `{Rep a A},
-      inv _ Empty nil
-  | inv_struct : forall `{Rep a A} (x:a) (q:queue (cat a)) X Ls L,
-      rep x X ->
-      @rep _ _ (@queue_rep _ _ (B)) q Ls ->
-      L =' X :: Ls ->
-      Forall (<> nil) Ls ->
-      inv _ (Struct x q) L.
-      
-(Rep := Build_Rep (@inv _ _ _))
+Section Polymorphic.
+Context `{Rep a A}.
 
-Global Instance deque_rep `{Rep a A} : Rep (cat a) (list A) :=
-  inv 0.
+Inductive inv : cat a -> list A -> Prop :=
+  | inv_empty : 
+      inv Empty nil
+  | inv_struct : forall (x:a) (q:queue (cat a)) X Ls L,
+      rep x X ->
+      Forall2 inv q Ls ->
+      L =' X :: concat Ls ->
+      Forall (<> nil) Ls ->
+      inv (Struct x q) L.
+      
+End Polymorphic.
+
+Global Instance cat_rep `{Rep a A} : Rep (cat a) (list A).
+Proof.
+  intros. apply (Build_Rep inv).
+  induction x; introv HX HY; inverts HX; inverts HY;
+   unfolds eq'; subst; try solve [prove_rep].
+  (*todo:inductino on size or depth ! *)
+skip.
+Defined.
 
 (** automation  *)
 
 Hint Constructors Forall2.
 Hint Resolve Forall2_last.
 Hint Extern 1 (@rep (cat _) _ _ _ _) => simpl.
-Hint Unfold inv.
+Hint Constructors inv.
 
-Ltac auto_tilde ::= eauto with maths.
+Ltac auto_tilde ::= eauto. (* with maths.*)
 
-Section Polymorphic.
+Section Polymorphic'.
 Variables (a A : Type) (RA:Rep a A).
 
   (* todo: avoid the following lines *)
-Hint Extern 1 (RegisterSpec Q.is_empty) => Provide (QS.is_empty_spec (H:=RA)).
-Hint Extern 1 (RegisterSpec Q.snoc) => Provide (QS.snoc_spec (H:=RA)).
-Hint Extern 1 (RegisterSpec Q.head) => Provide (QS.head_spec (H:=RA)).
-Hint Extern 1 (RegisterSpec Q.tail) => Provide (QS.tail_spec (H:=RA)).
+Hint Extern 1 (RegisterSpec Q.is_empty) => Provide (@QS.is_empty_spec (cats a) _ _).
+Hint Extern 1 (RegisterSpec Q.snoc) => Provide (@QS.snoc_spec (cats a) _ _).
+Hint Extern 1 (RegisterSpec Q.head) => Provide (@QS.head_spec (cats a) _ _).
+Hint Extern 1 (RegisterSpec Q.tail) => Provide (@QS.tail_spec (cats a) _ _).
 
 (** useful facts *)
 
 Lemma to_empty : forall L,
   rep Empty L -> L = nil.
-Proof. introv RL. inverts RL as _ M. inverts~ M. Qed.
+Proof. introv RL. inverts~ RL. Qed.
 
 Lemma to_not_empty : forall c L,
   rep c L -> L <> nil -> c <> Empty.
@@ -64,11 +85,7 @@ Qed.
 
 Lemma from_empty : forall c,
   rep c nil -> c = Empty.
-Proof.
-  introv RC. inverts RC as.
-  introv _ ID. inverts~ ID.
-  introv ? ? Df ? ? ?. inverts Df; false.
-Qed.
+Proof. introv RC. inverts RC. auto. false. Qed.
 
 (** verification *)
 
@@ -76,7 +93,7 @@ Lemma empty_spec :
   rep (@empty a) (@nil A).
 Proof.
   generalizes RA A. apply (empty_cf a). xgo.
-  intros. simpl. rew_list~.
+  intros. simple~.
 Qed.
 
 Hint Extern 1 (rep empty _) => apply empty_spec.
@@ -84,18 +101,24 @@ Hint Extern 1 (rep empty _) => apply empty_spec.
 Lemma is_empty_spec : 
   RepTotal is_empty (L;cat a) >> bool_of (L = nil).
 Proof.
-  xcf. intros (((lenf,f),lenr),r) Q RQ. xgo.
-  unfolds. extens. iff Z; fold_prop; subst.
-  apply~ empty_from_len.
-  intuit RQ. inverts H. destruct (nil_eq_app_rev_inv H5). subst~.
+  xcf. intros l L RL. xgo.
+  apply~ to_empty.
+  intro_subst_hyp. apply C. apply~ from_empty.
 Qed. 
 
 Hint Extern 1 (RegisterSpec is_empty) => Provide is_empty_spec.
+
+Hint Extern 1 (rep _ _) => simpl.
+Hint Resolve Forall_last.
 
 Lemma link_spec : 
   RepSpec link (L1;cat a) (L2;cat a) |R>>
     L1 <> nil -> L2 <> nil -> R (L1 ++ L2 ; cat a).
 Proof.
+  xcf. introv RL1 RL2 N1 N2. xmatch.
+  xgo. apply N1. apply~ to_empty.
+  inverts RL1. xapp~. xgo. simpls.
+  constructors~. subst. rew_concat; auto.  
 Qed.
 
 Hint Extern 1 (RegisterSpec link) => Provide link_spec.
@@ -104,6 +127,7 @@ Lemma link_all_spec :
   RepSpec link_all (Ls;queue (cat a)) |R>>
     Ls <> nil -> R (concat Ls ; cat a).
 Proof.
+  
 Qed.
 
 Hint Extern 1 (RegisterSpec link_all) => Provide link_all_spec.
