okasaki/QueueSig_proof.v
@@ -36,4 +36,43 @@ End QueueSigSpec.
 
 
 
+Definition rep_from_eq : forall A, Rep A A.
+Proof. intros. apply (Build_Rep eq). congruence. Defined.
+
+Module Type QueueBisSigSpec.
+
+Declare Module Q : MLQueueBis.
+Import Q.
+
+Definition queue_rep : forall `{Rep a A},  
+  Rep (queue a) (list A) 
+  := fun a A H => list_rep (H:=H).
+
+Existing Instance queue_rep. 
+
+Section Polymorphic.
+Variables (a A : Type) (RA:Rep a A).
+
+Parameter empty_spec : 
+  rep (@empty a) (@nil A).
+
+Parameter is_empty_spec : 
+  RepTotal is_empty (Q;queue a) >> bool_of (Q = nil).
+
+Parameter snoc_spec : 
+  RepTotal snoc (Q;queue a) (X;a) >> (Q&X) ; queue a.
+
+Parameter head_spec : 
+  RepSpec head (Q;queue a) |R>>
+     Q <> nil -> R (is_head Q ;; a).
+
+Parameter tail_spec :
+  RepSpec tail (Q;queue a) |R>> 
+     Q <> nil -> R (is_tail Q ;; queue a).
+
+End Polymorphic.
+
+End QueueBisSigSpec.
+
+
 
